doc/simple/coq/DeclInfra.v
@@ -24,106 +24,182 @@ Ltac exists_fresh :=
   let L := gather_vars_with (fun x : vars => x) in exists L.
 
 Scheme dtyping_induct := Induction for DTyping Sort Prop
-  with dwftyp_induct := Induction for DWfTyp Sort Prop
   with dwf_induct := Induction for DWf Sort Prop
-  with dinst_induct := Induction for DInst Sort Prop
-  with dgen_induct := Induction for DGen Sort Prop.
+  with dwf_subtyping := Induction for DSubtyping Sort Prop.
 
-Hint Constructors DRed DTyping DMode DWfTyp DWf DInst DGen.
+Hint Constructors DRed DTyping DMode DWf DSubtyping.
 
+Lemma dnotin_fv_fev: forall x t,
+    x \notin DFv t ->
+    x \notin DFev t
+with dnotin_tfv_tfev: forall x t,
+    x \notin DTFv t ->
+    x \notin DTFev t.
+Proof.
+  intros. induction t; simpls; auto.
+Proof.
+  intros. induction t; simpls; auto.
+Qed.
+
+Lemma dnotin_fv_ftv: forall x t,
+    x \notin DFv t ->
+    x \notin DFtv t
+with dnotin_tfv_tftv: forall x t,
+    x \notin DTFv t ->
+    x \notin DTFtv t.
+Proof.
+  intros. induction t; simpls; auto.
+Proof.
+  intros. induction t; simpls; auto.
+Qed.
+
+Lemma dnotin_fv_inv: forall x t,
+    x \notin DFev t -> x \notin DFtv t ->
+    x \notin DFv t
+with dnotin_tfv_inv: forall x t,
+    x \notin DTFev t -> x \notin DTFtv t ->
+    x \notin DTFv t.
+Proof.
+  intros. induction t; simpls; auto.
+Proof.
+  intros. induction t; simpls; auto.
+Qed.
+
+Hint Resolve dnotin_fv_fev dnotin_tfv_tfev dnotin_fv_ftv dnotin_tfv_tftv dnotin_fv_inv dnotin_tfv_inv.
 (** Substitution *)
 
-Hint Constructors DTerm.
+Hint Constructors DTerm DTermTy.
 
 (* Substitution on indices is identity on well-formed terms. *)
 
 Lemma dopen_rec_term_core :forall e j v i u, i <> j ->
-  DOpenRec j v e = DOpenRec i u (DOpenRec j v e) -> e = DOpenRec i u e.
+  DOpenRec j v e = DOpenRec i u (DOpenRec j v e) -> e = DOpenRec i u e
+with dopent_rec_term_core:forall e j v i u, i <> j ->
+  DOpenTypRec j v e = DOpenTypRec i u (DOpenTypRec j v e) -> e = DOpenTypRec i u e.
 Proof.
   induction e; introv Neq Equ;
   simpl in *; inversion* Equ; f_equal*.  
   case_nat*. case_nat*.
+Proof.
+  induction e; introv Neq Equ;
+  simpl in *; inversion* Equ; f_equal*.
 Qed.
 
 Lemma dtopen_rec_term_core :forall e j v i u, i <> j ->
-  DOpenTypRec j v e = DOpenTypRec i u (DOpenTypRec j v e) -> e = DOpenTypRec i u e.
+  DTOpenRec j v e = DTOpenRec i u (DTOpenRec j v e) -> e = DTOpenRec i u e
+with
+dtopent_rec_term_core :forall e j v i u, i <> j ->
+  DTOpenTypRec j v e = DTOpenTypRec i u (DTOpenTypRec j v e) -> e = DTOpenTypRec i u e.
 Proof.
   induction e; introv Neq Equ;
-    simpl in *; inversion* Equ; f_equal*.
-  apply dopen_rec_term_core with (j := j) (v := v).
-  auto. auto.
+  simpl in *; inversion* Equ; f_equal*.
+Proof.
+  induction e; introv Neq Equ;
+  simpl in *; inversion* Equ; f_equal*.
+  case_nat*. case_nat*.
+Qed.
+
+Lemma dopen_dtopen_rec_term_core :forall e j v i u, i <> j ->
+  DTOpenRec j v e = DOpenRec i u (DTOpenRec j v e) -> e = DOpenRec i u e
+with
+dopent_dtopent_rec_term_core :forall e j v i u, i <> j ->
+  DTOpenTypRec j v e = DOpenTypRec i u (DTOpenTypRec j v e) -> e = DOpenTypRec i u e.
+Proof.
+  induction e; introv Neq Equ;
+  simpl in *; inversion* Equ; f_equal*.
+Proof.
+  induction e; introv Neq Equ;
+  simpl in *; inversion* Equ; f_equal*.
+Qed.
+
+Lemma dtopen_dopen_rec_term_core :forall e j v i u, i <> j ->
+  DOpenRec j v e = DTOpenRec i u (DOpenRec j v e) -> e = DTOpenRec i u e
+with
+dtopent_dopent_rec_term_core :forall e j v i u, i <> j ->
+  DOpenTypRec j v e = DTOpenTypRec i u (DOpenTypRec j v e) -> e = DTOpenTypRec i u e.
+Proof.
+  induction e; introv Neq Equ;
+  simpl in *; inversion* Equ; f_equal*.
+Proof.
+  induction e; introv Neq Equ;
+  simpl in *; inversion* Equ; f_equal*.
 Qed.
 
 Lemma dopen_rec_term : forall t u,
-  DTerm t -> forall k, t = DOpenRec k u t.
+  DTerm t -> forall k, t = DOpenRec k u t
+with dopent_rec_term : forall t u,
+  DTermTy t -> forall k, t = DOpenTypRec k u t.
 Proof.
   induction 1; intros; simpl; f_equal*.
   unfolds DOpen. pick_fresh x.
    apply* (@dopen_rec_term_core e 0 (DE_FVar x)).
   unfolds DOpen. pick_fresh x.
-   apply* (@dopen_rec_term_core t2 0 (DE_FVar x)).
+   apply* (@dopent_rec_term_core t2 0 (DE_FVar x)).
   unfolds DOpen. pick_fresh x.
-   apply* (@dopen_rec_term_core e2 0 (DE_FVar x)).
+    apply* (@dopent_dtopent_rec_term_core t 0 (DT_TFVar x)).
+Proof.
+  induction 1; intros; simpl; f_equal*.
 Qed.
 
 Lemma dtopen_rec_term : forall t u,
-  DTermTy t -> forall k, t = DOpenTypRec k u t.
+  DTerm t -> forall k, t = DTOpenRec k u t
+with dtopent_rec_term : forall t u,
+  DTermTy t -> forall k, t = DTOpenTypRec k u t.
 Proof.
   induction 1; intros; simpl; f_equal*.
-  apply* dopen_rec_term.
-  unfolds DOpenT. pick_fresh x.
-   apply* (@dtopen_rec_term_core t 0 (DE_FVar x)).
+  unfolds DOpen. pick_fresh x.
+   apply* (@dtopen_dopen_rec_term_core e 0 (DE_FVar x)).
+  unfolds DOpen. pick_fresh x.
+   apply* (@dtopent_dopent_rec_term_core t2 0 (DE_FVar x)).
+  unfolds DOpen. pick_fresh x.
+   apply* (@dtopent_rec_term_core t 0 (DT_TFVar x)).
+Proof.
+  induction 1; intros; simpl; f_equal*.
 Qed.
 
-Lemma dopen_var_inj : forall x t1 t2, 
-  x \notin (DFv t1) -> x \notin (DFv t2) -> 
-  (t1 ^ x = t2 ^ x) -> (t1 = t2).
+Lemma dopen_var_inj : forall x t1 t2,
+  x \notin (DFv t1) -> x \notin (DFv t2) ->
+  forall k, (DOpenRec k (DE_FVar x) t1 = DOpenRec k (DE_FVar x) t2) -> (t1 = t2)
+with
+dtopen_var_inj : forall x t1 t2,
+  x \notin (DTFv t1) -> x \notin (DTFv t2) ->
+  forall k, (DOpenTypRec k (DE_FVar x) t1 = DOpenTypRec k (DE_FVar x) t2) -> (t1 = t2).
 Proof.
-  intros x t1. unfold DOpen. generalize 0.
-  induction t1; intro k; destruct t2; simpl; intros; inversion H1;
-  try solve [ f_equal* 
-  | do 2 try case_nat; inversions* H1; try notin_false ].
-Qed.
+  intros x t1.
+  induction t1; intro t2.
+  destruct t2; simpl; intros;try(case_nat~). case_nat~. case_nat~.
+  inversion H1; subst. notin_false.
+  destruct t2; simpl; intros; try(case_nat~); try(solve[inversion H1]).
+  inversion H1; subst. notin_false.
+  inversion H1; subst~.
+  destruct t2; simpl; intros; try(case_nat~); try(solve[inversion H1]); auto.
+  destruct t2; simpl; intros; try(case_nat~); try(solve[inversion H1]); auto.
+  inversion H1; subst. f_equal ~. apply* IHt1_1. apply* IHt1_2.
+  destruct t2; simpl; intros; try(case_nat~); try(solve[inversion H1]); auto.
+  inversion H1; subst. f_equal ~. apply* IHt1.
+  destruct t2; simpl; intros; try(case_nat~); try(solve[inversion H1]); auto.
+  inversion H1; subst. f_equal ~. apply* dtopen_var_inj. apply* dtopen_var_inj.
+  destruct t2; simpl; intros; try(case_nat~); try(solve[inversion H1]); auto.
+  inversion H1; subst. f_equal ~. apply* IHt1.
+  destruct t2; simpl; intros; try(case_nat~); try(solve[inversion H1]); auto.
+  inversion H1; subst. f_equal ~. apply* IHt1.
+  destruct t2; simpl; intros; try(case_nat~); try(solve[inversion H1]); auto.
+  inversion H1; subst. f_equal ~. apply* IHt1. apply* dtopen_var_inj.
+  destruct t2; simpl; intros; try(case_nat~); try(solve[inversion H1]); auto.
+  inversion H1; subst. f_equal ~. apply* dtopen_var_inj.
 
-Lemma notin_dopen_inv : forall x y n e,
-    x \notin DFv e ->
-    x \notin DFv y ->
-    x \notin DFv (DOpenRec n y e).
-Proof.
-  introv notin neq.
-  gen n. induction e; introv; simpls; auto.
-  case_if. auto. simpl.  auto.
-Qed.
-
-Lemma notin_dopen : forall x y e n,
-    x \notin (DFv (DOpenRec n y e)) ->
-    x \notin (DFv e).
-Proof.
-  introv notin. gen n.
-  induction e; introv notin; try(simpl in *; auto);
-    try(
-  apply notin_union in notin;
-  destruct notin as [notin1 notin2];
-  apply IHe1 in notin1;
-  apply IHe2 in notin2;
-  auto);
-    try(apply IHe in notin; auto).
+  intros x t1.
+  destruct t1; intros t2; destruct t2; simpl; intros; inversion H1; auto.
+  lets: dopen_var_inj H3; auto.
+  subst~.
 Qed.
 
 Lemma dopen_reorder: forall e1 e2 i j e,
     DTerm e1 ->
     DTerm e2 ->
     i <> j ->
-    DOpenRec i e1 (DOpenRec j e2 e) = DOpenRec j e2 (DOpenRec i e1 e).
-Proof.
-  introv te1 te2 neq.
-  gen i j. induction e; introv neq; simpls; auto; try(solve[f_equal ~]).
-  case_nat~. case_nat~. simpls. case_if~. symmetry. apply~ dopen_rec_term.
-  case_nat~. simpls. case_if~. apply~ dopen_rec_term.
-  simpls. case_if~. case_if~.
-Qed.
-
-Lemma dopent_reorder: forall e1 e2 i j e,
+    DOpenRec i e1 (DOpenRec j e2 e) = DOpenRec j e2 (DOpenRec i e1 e)
+with dopent_reorder: forall e1 e2 i j e,
     DTerm e1 ->
     DTerm e2 ->
     i <> j ->
@@ -131,115 +207,376 @@ Lemma dopent_reorder: forall e1 e2 i j e,
 Proof.
   introv te1 te2 neq.
   gen i j. induction e; introv neq; simpls; auto; try(solve[f_equal ~]).
-  f_equal. apply~ dopen_reorder.
-Qed.
-
-Lemma dopen_fv: forall n s y,
-    DTerm (DOpenRec n (DE_FVar y) s) ->
-    y \notin DFv (DOpenRec n (DE_FVar y) s) ->
-    DTerm s.
+  case_nat~. case_nat~. simpls. case_if~. symmetry. apply~ dopen_rec_term.
+  case_nat~. simpls. case_if~. apply~ dopen_rec_term.
+  simpls. case_if~. case_if~.
 Proof.
-  unfold DOpen.
-  introv dt.
-  gen_eq s2 : (DOpenRec n (DE_FVar y) s).
-  gen s n. induction dt; introv eq notin; simpls.
-
-  induction s; simpls; try(solve[inversion eq]).
-  case_nat*. inversion eq;  subst. false notin_same notin0.
-  apply DTerm_Var.
-
-  induction s; simpls; try(solve[inversion eq]).
-  case_nat*.
-  apply DTerm_Star.
-
-  induction s; simpls; try(solve[inversion eq]).
-  case_nat*.
-  inversion eq; subst.  apply DTerm_App; f_equal *.
-
-  induction s; simpls; try(solve[inversion eq]).
-  case_nat*.
-  inversion eq; subst.  apply DTerm_Lam with (L \u \{y}).
-  intros z notin_z. apply H0 with z (S n); auto. apply~ dopen_reorder.
-  apply~ notin_dopen_inv.
-  simpls. apply notin_singleton. auto_star.
-
-  induction s; simpls; try(solve[inversion eq]).
-  case_nat*.
-  inversion eq; subst.  apply DTerm_Pi with (L \u \{y}).
-  apply~ IHdt.
-  intros z notin_z. apply H0 with z (S n); auto. apply~ dopen_reorder.
-  apply~ notin_dopen_inv.
-  simpls. apply notin_singleton. auto_star.
-
-  induction s; simpls; try(solve[inversion eq]).
-  case_nat*.
-  inversion eq; subst.  apply DTerm_Let with (L \u \{y}).
-  apply~ IHdt.
-  intros z notin_z. apply H0 with z (S n); auto. apply~ dopen_reorder.
-  apply~ notin_dopen_inv.
-  simpls. apply notin_singleton. auto_star.
-
-  induction s; simpls; try(solve[inversion eq]).
-  case_nat*.
-  inversion eq; subst.  apply DTerm_CastUp; f_equal *.
-
-  induction s; simpls; try(solve[inversion eq]).
-  case_nat*.
-  inversion eq; subst.  apply DTerm_CastDn; f_equal *.
-
-  induction s; simpls; try(solve[inversion eq]).
-  case_nat*.
-  inversion eq; subst.  apply DTerm_Ann; f_equal *.
+  introv te1 te2 neq.
+  gen i j. induction e; introv neq; simpls; auto; try(solve[f_equal ~]).
 Qed.
 
-Lemma notin_dopent_inv : forall x y n e,
-    x \notin DTFv e ->
-    x \notin DFv y ->
-    x \notin DTFv (DOpenTypRec n y e).
+Lemma dtopen_reorder: forall e1 e2 i j e,
+    DTermTy e1 ->
+    DTermTy e2 ->
+    i <> j ->
+    DTOpenRec i e1 (DTOpenRec j e2 e) = DTOpenRec j e2 (DTOpenRec i e1 e)
+with
+dtopent_reorder: forall e1 e2 i j e,
+    DTermTy e1 ->
+    DTermTy e2 ->
+    i <> j ->
+    DTOpenTypRec i e1 (DTOpenTypRec j e2 e) = DTOpenTypRec j e2 (DTOpenTypRec i e1 e).
+Proof.
+  introv te1 te2 neq.
+  gen i j. induction e; introv neq; simpls; auto; try(solve[f_equal ~]).
+Proof.
+  introv te1 te2 neq.
+  gen i j. induction e; introv neq; simpls; auto; try(solve[f_equal ~]).
+  case_nat~. case_nat~. simpls. case_if~. symmetry. apply~ dtopent_rec_term.
+  case_nat~. simpls. case_if~. apply~ dtopent_rec_term.
+  simpls. case_if~. case_if~.
+Qed.
+
+Lemma notin_dopen_fev_inv : forall x y n e,
+    x \notin DFev e ->
+    x \notin DFev y ->
+    x \notin DFev (DOpenRec n y e)
+with notin_dopent_fev_inv : forall x y n e,
+    x \notin DTFev e ->
+    x \notin DFev y ->
+    x \notin DTFev (DOpenTypRec n y e).
 Proof.
   introv notin neq.
   gen n. induction e; introv; simpls; auto.
-  apply~ notin_dopen_inv.
+  case_if. auto. simpl.  auto.
+Proof.
+  introv notin neq.
+  gen n. induction e; introv; simpls; auto.
+Qed.
+
+Lemma notin_dopen_ftv_inv : forall x y n e,
+    x \notin DFtv e ->
+    x \notin DFtv y ->
+    x \notin DFtv (DOpenRec n y e)
+with notin_dopent_ftv_inv : forall x y n e,
+    x \notin DTFtv e ->
+    x \notin DFtv y ->
+    x \notin DTFtv (DOpenTypRec n y e).
+Proof.
+  introv notin neq.
+  gen n. induction e; introv; simpls; auto.
+  case_if. auto. simpl.  auto.
+Proof.
+  introv notin neq.
+  gen n. induction e; introv; simpls; auto.
+Qed.
+
+Lemma notin_dtopen_inv : forall x y n e,
+    x \notin DFv e ->
+    x \notin DTFv y ->
+    x \notin DFv (DTOpenRec n y e)
+with notin_dtopent_inv : forall x y n e,
+    x \notin DTFv e ->
+    x \notin DTFv y ->
+    x \notin DTFv (DTOpenTypRec n y e).
+Proof.
+  introv notin neq.
+  gen n. induction e; introv; simpls; auto.
+Proof.
+  introv notin neq.
+  gen n. induction e; introv; simpls; auto.
+  case_if. auto. simpl.  auto.
+Qed.
+
+Lemma notin_dopen_fev : forall x y e n,
+    x \notin (DFev (DOpenRec n y e)) ->
+    x \notin (DFev e)
+with
+notin_dopent_fev : forall x y e n,
+    x \notin (DTFev (DOpenTypRec n y e)) ->
+    x \notin (DTFev e).
+Proof.
+  introv notin. gen n.
+  induction e; introv notin; try(simpl in *; auto);
+  try(apply notin_union in notin;
+      destruct notin as [notin1 notin2];
+      apply IHe1 in notin1;
+      apply IHe2 in notin2; auto);
+  try(apply IHe in notin; auto);
+  try(apply notin_union in notin;
+      destruct notin as [notin1 notin2];
+      try(lets: notin_opent notin1);
+      try(lets: notin_opent notin2);
+      auto_star).
+  apply* notin_dopent_fev.
+Proof.
+  introv notin. gen n.
+  induction e; introv notin.
+    simpl in *; auto_star.
+    simpl in *. auto.
+    simpl in *. auto.
+    simpl in *. apply*  notin_dopen_fev.
+Qed.
+
+Lemma notin_dopen_ftv : forall x y e n,
+    x \notin (DFtv (DOpenRec n y e)) ->
+    x \notin (DFtv e)
+with
+notin_dopent_ftv : forall x y e n,
+    x \notin (DTFtv (DOpenTypRec n y e)) ->
+    x \notin (DTFtv e).
+Proof.
+  introv notin. gen n.
+  induction e; introv notin; try(simpl in *; auto);
+  try(apply notin_union in notin;
+      destruct notin as [notin1 notin2];
+      apply IHe1 in notin1;
+      apply IHe2 in notin2; auto);
+  try(apply IHe in notin; auto);
+  try(apply notin_union in notin;
+      destruct notin as [notin1 notin2];
+      try(lets: notin_opent notin1);
+      try(lets: notin_opent notin2);
+      auto_star).
+  apply* notin_dopent_ftv.
+Proof.
+  introv notin. gen n.
+  induction e; introv notin.
+    simpl in *; auto_star.
+    simpl in *. auto.
+    simpl in *. auto.
+    simpl in *. apply*  notin_dopen_ftv.
+Qed.
+
+Lemma notin_dtopen_ftv : forall x y e n,
+    x \notin (DFtv (DTOpenRec n y e)) ->
+    x \notin (DFtv e)
+with
+notin_dtopent_ftv : forall x y e n,
+    x \notin (DTFtv (DTOpenTypRec n y e)) ->
+    x \notin (DTFtv e).
+Proof.
+  introv notin. gen n.
+  induction e; introv notin; try(simpl in *; auto);
+  try(apply notin_union in notin;
+      destruct notin as [notin1 notin2];
+      apply IHe1 in notin1;
+      apply IHe2 in notin2; auto);
+  try(apply IHe in notin; auto);
+  try(apply notin_union in notin;
+      destruct notin as [notin1 notin2];
+      try(lets: notin_topen notin1);
+      try(lets: notin_topen notin2);
+      auto_star).
+  apply* notin_dtopent_ftv.
+Proof.
+  introv notin. gen n.
+  induction e; introv notin.
+    simpl in *; auto_star.
+    simpl in *. auto.
+    simpl in *. auto.
+    simpl in *. apply*  notin_dtopen_ftv.
+Qed.
+
+Lemma notin_dtopen_fev : forall x y e n,
+    x \notin (DFev (DTOpenRec n y e)) ->
+    x \notin (DFev e)
+with
+notin_dtopent_fev : forall x y e n,
+    x \notin (DTFev (DTOpenTypRec n y e)) ->
+    x \notin (DTFev e).
+Proof.
+  introv notin. gen n.
+  induction e; introv notin; try(simpl in *; auto);
+  try(apply notin_union in notin;
+      destruct notin as [notin1 notin2];
+      apply IHe1 in notin1;
+      apply IHe2 in notin2; auto);
+  try(apply IHe in notin; auto);
+  try(apply notin_union in notin;
+      destruct notin as [notin1 notin2];
+      try(lets: notin_topen notin1);
+      try(lets: notin_topen notin2);
+      auto_star).
+  apply* notin_dtopent_fev.
+
+  introv notin. gen n.
+  induction e; introv notin.
+    simpl in *; auto_star.
+    simpl in *. auto.
+    simpl in *. auto.
+    simpl in *. apply*  notin_dtopen_fev.
+Qed.
+
+Lemma notin_dopen_fv : forall x y e n,
+    x \notin (DFv (DOpenRec n y e)) ->
+    x \notin (DFv e)
+with
+notin_dopent_fv : forall x y e n,
+    x \notin (DTFv (DOpenTypRec n y e)) ->
+    x \notin (DTFv e).
+Proof.
+  intros. apply dnotin_fv_inv.
+  apply dnotin_fv_fev in H. apply* notin_dopen_fev.
+  apply dnotin_fv_ftv in H. apply* notin_dopen_ftv.
+Proof.
+  intros. apply dnotin_tfv_inv.
+  apply dnotin_tfv_tfev in H. apply* notin_dopent_fev.
+  apply dnotin_tfv_tftv in H. apply* notin_dopent_ftv.
+Qed.
+
+Lemma notin_dtopen_fv : forall x y e n,
+    x \notin (DFv (DTOpenRec n y e)) ->
+    x \notin (DFv e)
+with
+notin_dtopent_fv : forall x y e n,
+    x \notin (DTFv (DTOpenTypRec n y e)) ->
+    x \notin (DTFv e).
+Proof.
+  intros. apply dnotin_fv_inv.
+  apply dnotin_fv_fev in H. apply* notin_dtopen_fev.
+  apply dnotin_fv_ftv in H. apply* notin_dtopen_ftv.
+Proof.
+  intros. apply dnotin_tfv_inv.
+  apply dnotin_tfv_tfev in H. apply* notin_dtopent_fev.
+  apply dnotin_tfv_tftv in H. apply* notin_dtopent_ftv.
 Qed.
 
 (* Substitution for a fresh name is identity. *)
 
 Lemma dsubst_fresh : forall x t u, 
-  x \notin DFv t -> DSubst x u t = t.
-Proof.
-  intros. induction t; simpls; fequals*.
-  case_var*. 
-Qed.
-
-Lemma dtsubst_fresh : forall x t u, 
+  x \notin DFv t -> DSubst x u t = t
+with
+dtsubst_fresh : forall x t u,
   x \notin DTFv t -> DTSubst x u t = t.
 Proof.
   intros. induction t; simpls; fequals*.
-  apply* dsubst_fresh.
+  case_var*. 
+Proof.
+  intros. induction t; simpls; fequals*.
+Qed.
+
+Lemma dsubstt_fresh : forall x t u,
+  x \notin DFtv t -> DSubstT x u t = t
+with dtsubstt_fresh : forall x t u,
+  x \notin DTFtv t -> DTSubstT x u t = t.
+Proof.
+  intros. induction t; simpls; fequals*.
+Proof.
+  intros. induction t; simpls; fequals*.
+  case_var*.
 Qed.
 
 (* Substitution distributes on the open operation. *)
 
 Lemma dsubst_openrec : forall n x u t1 t2, DTerm u -> 
-  DSubst x u (DOpenRec n t2 t1) = DOpenRec n (DSubst x u t2) (DSubst x u t1).
+  DSubst x u (DOpenRec n t2 t1) = DOpenRec n (DSubst x u t2) (DSubst x u t1)
+with
+dtsubst_opentyprec : forall n x u t1 t2, DTerm u ->
+  DTSubst x u (DOpenTypRec n t2 t1) = DOpenTypRec n (DSubst x u t2) (DTSubst x u t1).
 Proof.
   intros. gen n.
   induction t1; intros; simpl; f_equal*.
   case_nat*. case_var*. apply* dopen_rec_term.
+Proof.
+  intros. induction t1; simpls; fequal *.
+Qed.
+
+Lemma dsubst_topenrec : forall n x u t1 t2, DTerm u ->
+  DSubst x u (DTOpenRec n t2 t1) = DTOpenRec n (DTSubst x u t2) (DSubst x u t1)
+with
+dtsubst_topentyprec : forall n x u t1 t2, DTerm u ->
+  DTSubst x u (DTOpenTypRec n t2 t1) = DTOpenTypRec n (DTSubst x u t2) (DTSubst x u t1).
+Proof.
+  intros. gen n.
+  induction t1; intros; simpl; f_equal*.
+  case_if*. apply* dtopen_rec_term.
+Proof.
+  intros. induction t1; simpls; fequal *.
+  case_nat*.
+Qed.
+
+Lemma dsubstt_openrec : forall n x u t1 t2, DTermTy u ->
+  DSubstT x u (DOpenRec n t2 t1) = DOpenRec n (DSubstT x u t2) (DSubstT x u t1)
+with
+dtsubstt_opentyprec : forall n x u t1 t2, DTermTy u ->
+  DTSubstT x u (DOpenTypRec n t2 t1) = DOpenTypRec n (DSubstT x u t2) (DTSubstT x u t1).
+Proof.
+  intros. gen n.
+  induction t1; intros; simpl; f_equal*.
+  case_nat*.
+Proof.
+  intros. induction t1; simpls; fequal *.
+  case_if*. apply* dopent_rec_term.
+Qed.
+
+Lemma dsubstt_topenrec : forall n x u t1 t2, DTermTy u ->
+  DSubstT x u (DTOpenRec n t2 t1) = DTOpenRec n (DTSubstT x u t2) (DSubstT x u t1)
+with
+dtsubstt_topentyprec : forall n x u t1 t2, DTermTy u ->
+  DTSubstT x u (DTOpenTypRec n t2 t1) = DTOpenTypRec n (DTSubstT x u t2) (DTSubstT x u t1).
+Proof.
+  intros. gen n.
+  induction t1; intros; simpl; f_equal*.
+Proof.
+  intros. induction t1; simpls; fequal *.
+  case_nat*.
+  case_if*. apply* dtopent_rec_term.
 Qed.
 
 Lemma dsubst_open : forall x u t1 t2, DTerm u -> 
-  DSubst x u (t1 ^^ t2) = (DSubst x u t1) ^^ (DSubst x u t2).
+  DSubst x u (t1 ^^ t2) = (DSubst x u t1) ^^ (DSubst x u t2)
+with dtsubst_open : forall x u t1 t2, DTerm u ->
+  DTSubst x u (t1 ^^' t2) = (DTSubst x u t1) ^^' (DSubst x u t2).
 Proof.
   intros. apply* dsubst_openrec.
-Qed.
-
-Lemma dtsubst_open : forall x u t1 t2, DTerm u -> 
-  DTSubst x u (t1 ^^' t2) = (DTSubst x u t1) ^^' (DSubst x u t2).
 Proof.
   intros. unfold DOpenT. generalize 0.
   induction t1; intros; simpl; f_equal*.
   apply* dsubst_openrec.
+Qed.
+
+Lemma dsubst_topen : forall x u t1 t2, DTerm u ->
+  DSubst x u (t1 ^^% t2) = (DSubst x u t1) ^^% (DTSubst x u t2)
+with
+  dtsubst_topen : forall x u t1 t2, DTerm u ->
+  DTSubst x u (t1 ^^%' t2) = (DTSubst x u t1) ^^%' (DTSubst x u t2).
+Proof.
+  intros. apply* dsubst_topenrec.
+Proof.
+  intros. unfold DOpenT. generalize 0.
+  induction t1; intros; simpl; f_equal*.
+  apply* dtsubst_topentyprec.
+  unfold DTOpenT. simpls. f_equal *.
+Qed.
+
+Lemma dsubstt_open : forall x u t1 t2, DTermTy u ->
+  DSubstT x u (t1 ^^ t2) = (DSubstT x u t1) ^^ (DSubstT x u t2)
+with
+  dtsubstt_open : forall x u t1 t2, DTermTy u ->
+  DTSubstT x u (t1 ^^' t2) = (DTSubstT x u t1) ^^' (DSubstT x u t2).
+Proof.
+  intros. apply* dsubstt_openrec.
+Proof.
+  intros. unfold DOpenT. generalize 0.
+  induction t1; intros; simpl; f_equal*.
+  case_if*. apply* dopent_rec_term.
+  apply* dsubstt_openrec.
+Qed.
+
+Lemma dsubstt_topen : forall x u t1 t2, DTermTy u ->
+  DSubstT x u (t1 ^^% t2) = (DSubstT x u t1) ^^% (DTSubstT x u t2)
+with
+  dtsubstt_topen : forall x u t1 t2, DTermTy u ->
+  DTSubstT x u (t1 ^^%' t2) = (DTSubstT x u t1) ^^%' (DTSubstT x u t2).
+Proof.
+  intros. apply* dsubstt_topenrec.
+Proof.
+  intros. unfold DOpenT. generalize 0.
+  induction t1; intros; simpl; f_equal*.
+  apply* dtsubstt_topentyprec.
+  case_if*. apply* dtopent_rec_term.
+  unfold DTOpenT. simpls. f_equal *.
 Qed.
 
 (* Substitution and open_var for distinct names commute. *)
@@ -255,6 +592,44 @@ Lemma dtsubst_open_var : forall x y u e, y <> x -> DTerm u ->
   (DTSubst x u e) ^' y = DTSubst x u (e ^' y).
 Proof.
   introv Neq Wu. rewrite* dtsubst_open.
+  simpl. case_var*.
+Qed.
+
+Lemma dsubst_open_tvar : forall x y u e, y <> x -> DTerm u ->
+  (DSubst x u e) ^% y = DSubst x u (e ^% y).
+Proof.
+  introv Neq Wu. rewrite* dsubst_topen.
+Qed.
+
+Lemma dtsubst_open_tvar : forall x y u e, y <> x -> DTerm u ->
+  (DTSubst x u e) ^%' y = DTSubst x u (e ^%' y).
+Proof.
+  introv Neq Wu. rewrite* dtsubst_topen.
+Qed.
+
+Lemma dsubstt_open_var : forall x y u e, y <> x -> DTermTy u ->
+  (DSubstT x u e) ^ y = DSubstT x u (e ^ y).
+Proof.
+  introv Neq Wu. rewrite* dsubstt_open.
+Qed.
+
+Lemma dtsubstt_open_var : forall x y u e, y <> x -> DTermTy u ->
+  (DTSubstT x u e) ^' y = DTSubstT x u (e ^' y).
+Proof.
+  introv Neq Wu. rewrite* dtsubstt_open.
+Qed.
+
+Lemma dsubstt_open_tvar : forall x y u e, y <> x -> DTermTy u ->
+  (DSubstT x u e) ^% y = DSubstT x u (e ^% y).
+Proof.
+  introv Neq Wu. rewrite* dsubstt_topen.
+  simpl. case_var*.
+Qed.
+
+Lemma dtsubstt_open_tvar : forall x y u e, y <> x -> DTermTy u ->
+  (DTSubstT x u e) ^%' y = DTSubstT x u (e ^%' y).
+Proof.
+  introv Neq Wu. rewrite* dtsubstt_topen.
   simpl. case_var*.
 Qed.
 
@@ -277,6 +652,22 @@ Proof.
   rewrite* dtsubst_fresh. simpl. case_var*.
 Qed.
 
+Lemma dsubstt_intro : forall x t u,
+  x \notin (DFv t) -> DTermTy u ->
+  t ^^% u = DSubstT x u (t ^% x).
+Proof.
+  introv Fr Wu. rewrite* dsubstt_topen.
+  rewrite* dsubstt_fresh. simpl. case_var*.
+Qed.
+
+Lemma dtsubstt_intro : forall x t u,
+  x \notin (DTFv t) -> DTermTy u ->
+  t ^^%' u = DTSubstT x u (t ^%' x).
+Proof.
+  introv Fr Wu. rewrite* dtsubstt_topen.
+  rewrite* dtsubstt_fresh. simpl. case_var*.
+Qed.
+
 (* Tactic to permute subst and open var *)
 
 Ltac cross := 
@@ -296,21 +687,32 @@ Tactic Notation "crosst" "*" :=
 (* Terms are stable by substitution *)
 
 Lemma dsubst_term : forall t z u,
-  DTerm u -> DTerm t -> DTerm (DSubst z u t).
+  DTerm u -> DTerm t -> DTerm (DSubst z u t)
+with
+dtsubst_term : forall t z u,
+  DTerm u -> DTermTy t -> DTermTy (DTSubst z u t)
+with
+dsubstt_term : forall t z u,
+  DTermTy u -> DTerm t -> DTerm (DSubstT z u t)
+with
+dtsubstt_term : forall t z u,
+  DTermTy u -> DTermTy t -> DTermTy (DTSubstT z u t).
 Proof.
   induction 2; simple*.
   case_var*.
   apply_fresh* DTerm_Lam as y. rewrite* dsubst_open_var.
-  apply_fresh* DTerm_Pi as y. rewrite* dsubst_open_var.
-  apply_fresh* DTerm_Let as y. rewrite* dsubst_open_var.
-Qed.
-
-Lemma dtsubst_term : forall t z u,
-  DTerm u -> DTermTy t -> DTermTy (DTSubst z u t).
+  apply_fresh* DTerm_Pi as y. rewrite* dtsubst_open_var.
+  apply_fresh* DTerm_Forall as y. rewrite* dtsubst_open_tvar.
 Proof.
   induction 2; simple*.
-  apply* DTermTy_Expr. apply* dsubst_term.
-  apply_fresh* DTermTy_Forall as y. rewrite* dtsubst_open_var.
+Proof.
+  induction 2; simple*.
+  apply_fresh* DTerm_Lam as y. rewrite* dsubstt_open_var.
+  apply_fresh* DTerm_Pi as y. rewrite* dtsubstt_open_var.
+  apply_fresh* DTerm_Forall as y. rewrite* dtsubstt_open_tvar.
+Proof.
+  induction 2; simple*.
+  case_var*.
 Qed.
 
 (* Terms are stable by open *)
@@ -340,33 +742,15 @@ Proof.
 Qed.
 
 Lemma dbody_pi : forall t1 t2,
-  DTerm (DE_Pi t1 t2) -> DBody t2.
+  DTerm (DE_Pi t1 t2) -> DBodyTy t2.
 Proof.
-  intros. unfold DBody. inversion* H.
-Qed.
-
-Lemma dbody_let : forall e1 e2,
-  DTerm (DE_Let e1 e2) -> DBody e2.
-Proof.
-  intros. unfold DBody. inversion* H.
+  intros. unfold DBodyTy. inversion* H.
 Qed.
 
 Lemma dterm_pi : forall t1 t2,
-  DTerm (DE_Pi t1 t2) -> DTerm t1.
+  DTerm (DE_Pi t1 t2) -> DTermTy t1.
 Proof.
   intros. inversion* H.
-Qed.
-
-Lemma dterm_let : forall e1 e2,
-  DTerm (DE_Let e1 e2) -> DTerm e1.
-Proof.
-  intros. inversion* H.
-Qed.
-
-Lemma dtermty_forall : forall e,
-  DTermTy (DT_Forall e) -> DBodyTy e.
-Proof.
-  intros. unfold DBodyTy. inversions* H.
 Qed.
 
 Lemma dtermty_expr : forall e,
@@ -378,15 +762,12 @@ Qed.
 Hint Extern 1 (DTerm ?t) =>
   match goal with
   | H: DTerm (DE_Pi t ?t2) |- _ => apply (@dterm_pi t2)
-  | H: DTerm (DE_Let t ?t2) |- _ => apply (@dterm_let t2)
   | H: DTerm (DT_Expr ?t2) |- _ => apply (@dtermty_expr t2)
   end.
 
 Hint Extern 3 (DBody ?t) =>
   match goal with 
   | H: context [DE_Lam t] |- _ => apply (@dbody_lam)
-  | H: context [DE_Pi ?t1 t] |- _ => apply (@dbody_pi t1)
-  | H: context [DE_Let ?t1 t] |- _ => apply (@dbody_let t1)
   end.
 
 Hint Extern 1 (DBody ?t) =>
@@ -401,7 +782,7 @@ Hint Extern 1 (DBody ?t) =>
 
 Hint Extern 3 (DBodyTy ?t) =>
   match goal with 
-  | H: context [DT_Forall t] |- _ => apply (@dtermty_forall)
+  | H: context [DE_Pi t] |- _ => apply (@dbody_pi)
   end.
 
 Hint Extern 1 (DBodyTy ?t) =>
@@ -422,21 +803,17 @@ Proof.
 Qed.
 
 Lemma dterm_pi_prove : forall t1 t2,
-  DTerm t1 -> DBody t2 -> DTerm (DE_Pi t1 t2).
+  DTermTy t1 -> DBodyTy t2 -> DTerm (DE_Pi t1 t2).
 Proof.
   intros. apply_fresh* DTerm_Pi as x.
 Qed.
 
-Lemma dterm_let_prove : forall e1 e2,
-  DTerm e1 -> DBody e2 -> DTerm (DE_Let e1 e2).
-Proof.
-  intros. apply_fresh* DTerm_Let as x.
-Qed.
-
 Lemma dtermty_forall_prove : forall s,
-  DBodyTy s -> DTermTy (DT_Forall s).
+  DTermTy s -> DTerm (DE_Forall s).
 Proof.
-  intros. apply_fresh* DTermTy_Forall as x.
+  intros. apply_fresh* DTerm_Forall as x.
+  inversion H. unfold DTOpenT. simpls. apply* DTermTy_TFVar.
+  unfold DTOpenT. simpls. apply DTermTy_Expr. rewrite <- dtopen_rec_term; auto.
 Qed.
 
 Lemma dtermty_expr_prove : forall e,
@@ -446,7 +823,7 @@ Proof.
 Qed.
 
 Hint Resolve dterm_lam_prove
-     dterm_pi_prove dterm_let_prove
+     dterm_pi_prove
      dtermty_forall_prove dtermty_expr_prove.
 
 Lemma dbody_prove : forall L t,
@@ -496,8 +873,6 @@ Hint Resolve dbodyty_subst.
 Lemma dred_regular : forall t t', DRed t t' -> DTerm t /\ DTerm t'.
 Proof.
   intros_all. induction* H.
-  split*. apply* dopen_term.
-  apply* dterm_let.
 Qed.
 
 Hint Extern 1 (DTerm ?t) => match goal with
@@ -513,584 +888,371 @@ Hint Extern 1 (DTerm (DE_Pi (DSubst ?x ?u ?t1) (DSubst ?x ?u ?t2))) =>
   match goal with H: DTerm (DE_Pi t1 t2) |- _ => 
   unsimpl (DSubst x u (DE_Pi t1 t2)) end.
 
-Hint Extern 1 (DTerm (DE_Let (DSubst ?x ?u ?t1) (DSubst ?x ?u ?t2))) =>
-  match goal with H: DTerm (DE_Let t1 t2) |- _ => 
-  unsimpl (DSubst x u (DE_Let t1 t2)) end.
+Hint Extern 1 (DTerm (DE_Forall (DTSubst ?x ?u ?t2))) =>
+  match goal with H: DTermTy (DE_Forall t2) |- _ =>
+  unsimpl (DTSubst x u (DE_Forall t2)) end.
 
-Hint Extern 1 (DTermTy (DT_Forall (DTSubst ?x ?u ?t2))) =>
-  match goal with H: DTermTy (DT_Forall t2) |- _ => 
-  unsimpl (DTSubst x u (DT_Forall t2)) end.
+(* Definition contains_terms (E : DCtx) := *)
+(*   (forall x U, binds x (DC_Typ U) E -> DTerm U) /\ *)
+(*   (forall x T U, binds x (DC_Bnd T U) E -> DTermTy T /\ DTerm U). *)
 
-Definition contains_terms (E : DCtx) :=
-  (forall x U, binds x (DC_Typ U) E -> DTerm U) /\
-  (forall x T U, binds x (DC_Bnd T U) E -> DTermTy T /\ DTerm U).
-
-Lemma regular_dtyping : forall m E t T, DTyping m E t T ->
-  (DWf E /\ ok E /\ contains_terms E /\ DTerm t /\ DTerm T).
-Proof.
-  apply dtyping_induct with
-  (P0 := fun E t (_ : DWfTyp E t) => DWf E /\ ok E /\ contains_terms E /\ DTermTy t)
-  (P1 := fun E (_ : DWf E) => ok E /\ contains_terms E)
-  (P2 := fun E t T (_ : DInst E t T) => DWf E /\ ok E /\ contains_terms E /\ DTerm T)
-  (P3 := fun E t T(_ : DGen E t T) => DWf E /\ ok E /\ contains_terms E /\ DTerm t /\ DTermTy T); 
-    unfolds contains_terms; intros; splits*.
+(* Lemma regular_dtyping : forall m E t T, DTyping m E t T -> *)
+(*   (DWf E /\ ok E /\ contains_terms E /\ DTerm t /\ DTerm T). *)
+(* Proof. *)
+(*   apply dtyping_induct with *)
+(*   (P0 := fun E t (_ : DWfTyp E t) => DWf E /\ ok E /\ contains_terms E /\ DTermTy t) *)
+(*   (P1 := fun E (_ : DWf E) => ok E /\ contains_terms E) *)
+(*   (P2 := fun E t T (_ : DInst E t T) => DWf E /\ ok E /\ contains_terms E /\ DTerm T) *)
+(*   (P3 := fun E t T(_ : DGen E t T) => DWf E /\ ok E /\ contains_terms E /\ DTerm t /\ DTermTy T);  *)
+(*     unfolds contains_terms; intros; splits*. *)
   
-  pick_fresh x. assert (x \notin L) by auto.
-  destruct (H x H0) as [H1 [_ [_ _]]].
-  inversion* H1. false* empty_push_inv.
-  destruct (eq_push_inv H2) as [_ [_ Eq]]. subst*.
-  destruct (eq_push_inv H2) as [_ [_ Eq]]. subst*.
-  destruct (eq_push_inv H2) as [_ [_ Eq]]. subst*.
+(*   pick_fresh x. assert (x \notin L) by auto. *)
+(*   destruct (H x H0) as [H1 [_ [_ _]]]. *)
+(*   inversion* H1. false* empty_push_inv. *)
+(*   destruct (eq_push_inv H2) as [_ [_ Eq]]. subst*. *)
+(*   destruct (eq_push_inv H2) as [_ [_ Eq]]. subst*. *)
+(*   destruct (eq_push_inv H2) as [_ [_ Eq]]. subst*. *)
 
-  pick_fresh x. assert (x \notin L) by auto.
-  destruct~ (H x H0) as [_ [H1 [_ _]]].
+(*   pick_fresh x. assert (x \notin L) by auto. *)
+(*   destruct~ (H x H0) as [_ [H1 [_ _]]]. *)
 
-  split; intros.
-  pick_fresh y. assert (y \notin L) by auto.
-  destruct~ (H y H1) as [_ [_ [[H2 _] _]]].
-  apply* (H2 x U).
-  pick_fresh y. assert (y \notin L) by auto.
-  destruct~ (H y H1) as [_ [_ [[_ H2] _]]].
-  apply* (H2 x T U).
+(*   split; intros. *)
+(*   pick_fresh y. assert (y \notin L) by auto. *)
+(*   destruct~ (H y H1) as [_ [_ [[H2 _] _]]]. *)
+(*   apply* (H2 x U). *)
+(*   pick_fresh y. assert (y \notin L) by auto. *)
+(*   destruct~ (H y H1) as [_ [_ [[_ H2] _]]]. *)
+(*   apply* (H2 x T U). *)
   
-  intros. false* binds_empty_inv.
-  intros. false* binds_empty_inv.
+(*   intros. false* binds_empty_inv. *)
+(*   intros. false* binds_empty_inv. *)
 
-  intros. destruct (binds_push_inv H1) as [[? ?]|[? ?]].
-  injection H3; intros. subst*.
-  destruct H as [_ [H4 _]].
-  apply H4 with (x := x0). auto.
+(*   intros. destruct (binds_push_inv H1) as [[? ?]|[? ?]]. *)
+(*   injection H3; intros. subst*. *)
+(*   destruct H as [_ [H4 _]]. *)
+(*   apply H4 with (x := x0). auto. *)
 
-  intros. destruct (binds_push_inv H1) as [[? ?]|[? ?]].
-  false*. destruct H as [_ [_ H4]].
-  apply H4 with (x := x0). auto.
+(*   intros. destruct (binds_push_inv H1) as [[? ?]|[? ?]]. *)
+(*   false*. destruct H as [_ [_ H4]]. *)
+(*   apply H4 with (x := x0). auto. *)
 
-  intros. destruct (binds_push_inv H2) as [[? ?]|[? ?]].
-  false*. destruct H as [_ [H5 _]].
-  apply H5 with (x := x0). auto.
+(*   intros. destruct (binds_push_inv H2) as [[? ?]|[? ?]]. *)
+(*   false*. destruct H as [_ [H5 _]]. *)
+(*   apply H5 with (x := x0). auto. *)
 
-  intros. destruct (binds_push_inv H2) as [[? ?]|[? ?]].
-  injection H4; intros. subst*.
-  destruct H as [_ [_ H5]].
-  apply H5 with (x := x0). auto.
+(*   intros. destruct (binds_push_inv H2) as [[? ?]|[? ?]]. *)
+(*   injection H4; intros. subst*. *)
+(*   destruct H as [_ [_ H5]]. *)
+(*   apply H5 with (x := x0). auto. *)
 
-  intros. destruct (binds_push_inv H2) as [[? ?]|[? ?]].
-  false*. destruct H as [_ [H5 _]].
-  apply H5 with (x := x0). auto.
+(*   intros. destruct (binds_push_inv H2) as [[? ?]|[? ?]]. *)
+(*   false*. destruct H as [_ [H5 _]]. *)
+(*   apply H5 with (x := x0). auto. *)
 
-  intros. destruct (binds_push_inv H2) as [[? ?]|[? ?]].
-  injection H4; intros. subst*.
-  pick_fresh y. assert (y \notin L) by auto.
-  destruct (H1 y H3) as [_ [_ H5]].
-  destruct (H5 x (s ^' y) t). auto. split*.
-  destruct H as [_ [_ H5]].
-  apply H5 with (x := x0). auto.
+(*   intros. destruct (binds_push_inv H2) as [[? ?]|[? ?]]. *)
+(*   injection H4; intros. subst*. *)
+(*   pick_fresh y. assert (y \notin L) by auto. *)
+(*   destruct (H1 y H3) as [_ [_ H5]]. *)
+(*   destruct (H5 x (s ^' y) t). auto. split*. *)
+(*   destruct H as [_ [_ H5]]. *)
+(*   apply H5 with (x := x0). auto. *)
 
-  pick_fresh x. assert (x \notin L) by auto.
-  assert (x \notin DFv e) by auto.
-  destruct (H x H0 H1) as [H2 [_ [_ _]]].
-  inversion* H2. false* empty_push_inv.
-  destruct (eq_push_inv H3) as [_ [_ Eq]]. subst*.
-  destruct (eq_push_inv H3) as [_ [_ Eq]]. subst*.
-  destruct (eq_push_inv H3) as [_ [_ Eq]]. subst*.
+(*   pick_fresh x. assert (x \notin L) by auto. *)
+(*   assert (x \notin DFv e) by auto. *)
+(*   destruct (H x H0 H1) as [H2 [_ [_ _]]]. *)
+(*   inversion* H2. false* empty_push_inv. *)
+(*   destruct (eq_push_inv H3) as [_ [_ Eq]]. subst*. *)
+(*   destruct (eq_push_inv H3) as [_ [_ Eq]]. subst*. *)
+(*   destruct (eq_push_inv H3) as [_ [_ Eq]]. subst*. *)
 
-  pick_fresh x. assert (x \notin L) by auto.
-  assert (x \notin DFv e) by auto.
-  destruct~ (H x H0 H1) as [_ [H2 [_ _]]].
+(*   pick_fresh x. assert (x \notin L) by auto. *)
+(*   assert (x \notin DFv e) by auto. *)
+(*   destruct~ (H x H0 H1) as [_ [H2 [_ _]]]. *)
 
-  split; intros.
-  pick_fresh y. assert (y \notin L) by auto.
-  assert (y \notin DFv e) by auto.
-  destruct~ (H y H1 H2) as [_ [_ [[H3 _] _]]].
-  apply* (H3 x U).
-  pick_fresh y. assert (y \notin L) by auto.
-  assert (y \notin DFv e) by auto.
-  destruct~ (H y H1 H2) as [_ [_ [[_ H3] _]]].
-  apply* (H3 x T U).
+(*   split; intros. *)
+(*   pick_fresh y. assert (y \notin L) by auto. *)
+(*   assert (y \notin DFv e) by auto. *)
+(*   destruct~ (H y H1 H2) as [_ [_ [[H3 _] _]]]. *)
+(*   apply* (H3 x U). *)
+(*   pick_fresh y. assert (y \notin L) by auto. *)
+(*   assert (y \notin DFv e) by auto. *)
+(*   destruct~ (H y H1 H2) as [_ [_ [[_ H3] _]]]. *)
+(*   apply* (H3 x T U). *)
   
-  pick_fresh x. assert (x \notin L) by auto.
-  assert (x \notin DFv e) by auto.
-  destruct~ (H x H0 H1) as [_ [_ [_ [H2 _]]]].
-Qed.
+(*   pick_fresh x. assert (x \notin L) by auto. *)
+(*   assert (x \notin DFv e) by auto. *)
+(*   destruct~ (H x H0 H1) as [_ [_ [_ [H2 _]]]]. *)
+(* Qed. *)
 
-Lemma open_var_inj : forall x t1 t2,
-  x \notin (DFv t1) -> x \notin (DFv t2) ->
-  (t1 ^ x = t2 ^ x) -> (t1 = t2).
-Proof.
-  intros x t1. unfold DOpen. generalize 0.
-  induction t1; intro k; destruct t2; simpl; intros; inversion H1;
-  try solve [ f_equal*
-  | do 2 try case_nat; inversions* H1; try notin_false ].
-Qed.
 
-Lemma openrec_var_inj : forall x t1 k t2,
-  x \notin (DFv t1) -> x \notin (DFv t2) ->
-  (DOpenRec k (DE_FVar x) t1 = DOpenRec k (DE_FVar x) t2) -> (t1 = t2).
-Proof.
-  intros x t1. unfold DOpenRec.
-  induction t1; intro k; destruct t2; simpl; intros; inversion H1;
-  try solve [ f_equal*
-  | do 2 try case_nat; inversions* H1; try notin_false ].
-Qed.
-
-Lemma opent_var_inj : forall x t1 t2,
-  x \notin (DTFv t1) -> x \notin (DTFv t2) ->
-  (t1 ^' x = t2 ^' x) -> (t1 = t2).
-Proof.
-  intros x t1. unfold DOpenT. generalize 0.
-  induction t1; intro k; destruct t2; simpl; intros; inversion H1;
-  try solve [ f_equal*
-  | do 2 try case_nat; inversions* H1; try notin_false ].
-
-  assert(d = d0). apply* openrec_var_inj.
-  subst*.
-Qed.
-
-Lemma regular_dinst : forall E s t, DInst E s t ->
-  (DWf E /\ ok E /\ contains_terms E /\ DTerm t).
-Proof.
-  apply dinst_induct with
-  (P := fun m E t T (_ : DTyping m E t T) => DWf E /\ ok E /\ contains_terms E /\ DTerm t /\ DTerm T)
-  (P0 := fun E t (_ : DWfTyp E t) => DWf E /\ ok E /\ contains_terms E /\ DTermTy t)
-  (P1 := fun E (_ : DWf E) => ok E /\ contains_terms E)
-  (P3 := fun E t T(_ : DGen E t T) => DWf E /\ ok E /\ contains_terms E /\ DTerm t /\ DTermTy T); 
-    unfolds contains_terms; intros; splits*.
+(* Lemma regular_dwftyp : forall E t, DWfTyp E t -> *)
+(*   (DWf E /\ ok E /\ contains_terms E /\ DTermTy t). *)
+(* Proof. *)
+(*   apply dwftyp_induct with *)
+(*   (P := fun m E t T (_ : DTyping m E t T) => DWf E /\ ok E /\ contains_terms E /\ DTerm t /\ DTerm T) *)
+(*   (P1 := fun E (_ : DWf E) => ok E /\ contains_terms E) *)
+(*   (P2 := fun E t T (_ : DInst E t T) => DWf E /\ ok E /\ contains_terms E /\ DTerm T) *)
+(*   (P3 := fun E t T(_ : DGen E t T) => DWf E /\ ok E /\ contains_terms E /\ DTerm t /\ DTermTy T);  *)
+(*     unfolds contains_terms; intros; splits*. *)
   
-  pick_fresh x. assert (x \notin L) by auto.
-  destruct (H x H0) as [H1 [_ [_ _]]].
-  inversion* H1. false* empty_push_inv.
-  destruct (eq_push_inv H2) as [_ [_ Eq]]. subst*.
-  destruct (eq_push_inv H2) as [_ [_ Eq]]. subst*.
-  destruct (eq_push_inv H2) as [_ [_ Eq]]. subst*.
+(*   pick_fresh x. assert (x \notin L) by auto. *)
+(*   destruct (H x H0) as [H1 [_ [_ _]]]. *)
+(*   inversion* H1. false* empty_push_inv. *)
+(*   destruct (eq_push_inv H2) as [_ [_ Eq]]. subst*. *)
+(*   destruct (eq_push_inv H2) as [_ [_ Eq]]. subst*. *)
+(*   destruct (eq_push_inv H2) as [_ [_ Eq]]. subst*. *)
 
-  pick_fresh x. assert (x \notin L) by auto.
-  destruct~ (H x H0) as [_ [H1 [_ _]]].
+(*   pick_fresh x. assert (x \notin L) by auto. *)
+(*   destruct~ (H x H0) as [_ [H1 [_ _]]]. *)
 
-  split; intros.
-  pick_fresh y. assert (y \notin L) by auto.
-  destruct~ (H y H1) as [_ [_ [[H2 _] _]]].
-  apply* (H2 x U).
-  pick_fresh y. assert (y \notin L) by auto.
-  destruct~ (H y H1) as [_ [_ [[_ H2] _]]].
-  apply* (H2 x T U).
+(*   split; intros. *)
+(*   pick_fresh y. assert (y \notin L) by auto. *)
+(*   destruct~ (H y H1) as (_ & _ & (H2 & _) & _). *)
+(*   apply* (H2 x U). *)
+(*   pick_fresh y. assert (y \notin L) by auto. *)
+(*   destruct~ (H y H1) as (_ & _ & (_ & H2) & _). *)
+(*   apply* (H2 x T U).  *)
   
-  intros. false* binds_empty_inv.
-  intros. false* binds_empty_inv.
+(*   intros. false* binds_empty_inv. *)
+(*   intros. false* binds_empty_inv. *)
 
-  intros. destruct (binds_push_inv H1) as [[? ?]|[? ?]].
-  injection H3; intros. subst*.
-  destruct H as [_ [H4 _]].
-  apply H4 with (x := x0). auto.
+(*   intros. destruct (binds_push_inv H1) as [[? ?]|[? ?]]. *)
+(*   injection H3; intros. subst*. *)
+(*   destruct H as [_ [H4 _]]. *)
+(*   apply H4 with (x := x0). auto. *)
 
-  intros. destruct (binds_push_inv H1) as [[? ?]|[? ?]].
-  false*. destruct H as [_ [_ H4]].
-  apply H4 with (x := x0). auto.
+(*   intros. destruct (binds_push_inv H1) as [[? ?]|[? ?]]. *)
+(*   false*. destruct H as [_ [_ H4]]. *)
+(*   apply H4 with (x := x0). auto. *)
 
-  intros. destruct (binds_push_inv H2) as [[? ?]|[? ?]].
-  false*. destruct H as [_ [H5 _]].
-  apply H5 with (x := x0). auto.
+(*   intros. destruct (binds_push_inv H2) as [[? ?]|[? ?]]. *)
+(*   false*. destruct H as [_ [H5 _]]. *)
+(*   apply H5 with (x := x0). auto. *)
 
-  intros. destruct (binds_push_inv H2) as [[? ?]|[? ?]].
-  injection H4; intros. subst*.
-  destruct H as [_ [_ H5]].
-  apply H5 with (x := x0). auto.
+(*   intros. destruct (binds_push_inv H2) as [[? ?]|[? ?]]. *)
+(*   injection H4; intros. subst*. *)
+(*   destruct H as [_ [_ H5]]. *)
+(*   apply H5 with (x := x0). auto. *)
 
-  intros. destruct (binds_push_inv H2) as [[? ?]|[? ?]].
-  false*. destruct H as [_ [H5 _]].
-  apply H5 with (x := x0). auto.
+(*   intros. destruct (binds_push_inv H2) as [[? ?]|[? ?]]. *)
+(*   false*. destruct H as [_ [H5 _]]. *)
+(*   apply H5 with (x := x0). auto. *)
 
-  intros. destruct (binds_push_inv H2) as [[? ?]|[? ?]].
-  injection H4; intros. subst*.
-  pick_fresh y. assert (y \notin L) by auto.
-  destruct (H1 y H3) as [_ [_ H5]].
-  destruct (H5 x (s ^' y) t). auto. split*.
-  destruct H as [_ [_ H5]].
-  apply H5 with (x := x0). auto.
+(*   intros. destruct (binds_push_inv H2) as [[? ?]|[? ?]]. *)
+(*   injection H4; intros. subst*. *)
+(*   pick_fresh y. assert (y \notin L) by auto. *)
+(*   destruct (H1 y H3) as [_ [_ H5]]. *)
+(*   destruct (H5 x (s ^' y) t). auto. split*. *)
+(*   destruct H as [_ [_ H5]]. *)
+(*   apply H5 with (x := x0). auto. *)
 
-  pick_fresh x. assert (x \notin L) by auto.
-  assert (x \notin DFv e) by auto.
-  destruct (H x H0 H1) as [H2 [_ [_ _]]].
-  inversion* H2. false* empty_push_inv.
-  destruct (eq_push_inv H3) as [_ [_ Eq]]. subst*.
-  destruct (eq_push_inv H3) as [_ [_ Eq]]. subst*.
-  destruct (eq_push_inv H3) as [_ [_ Eq]]. subst*.
+(*   pick_fresh x. assert (x \notin L) by auto. *)
+(*   assert (x \notin DFv e) by auto. *)
+(*   destruct (H x H0 H1) as [H2 [_ [_ _]]]. *)
+(*   inversion* H2. false* empty_push_inv. *)
+(*   destruct (eq_push_inv H3) as [_ [_ Eq]]. subst*. *)
+(*   destruct (eq_push_inv H3) as [_ [_ Eq]]. subst*. *)
+(*   destruct (eq_push_inv H3) as [_ [_ Eq]]. subst*. *)
 
-  pick_fresh x. assert (x \notin L) by auto.
-  assert (x \notin DFv e) by auto.
-  destruct~ (H x H0 H1) as [_ [H2 [_ _]]].
+(*   pick_fresh x. assert (x \notin L) by auto. *)
+(*   assert (x \notin DFv e) by auto. *)
+(*   destruct~ (H x H0 H1) as [_ [H2 [_ _]]]. *)
 
-  split; intros.
-  pick_fresh y. assert (y \notin L) by auto.
-  assert (y \notin DFv e) by auto.
-  destruct~ (H y H1 H2) as [_ [_ [[H3 _] _]]].
-  apply* (H3 x U).
-  pick_fresh y. assert (y \notin L) by auto.
-  assert (y \notin DFv e) by auto.
-  destruct~ (H y H1 H2) as [_ [_ [[_ H3] _]]].
-  apply* (H3 x T U).
+(*   split; intros. *)
+(*   pick_fresh y. assert (y \notin L) by auto. *)
+(*   assert (y \notin DFv e) by auto. *)
+(*   destruct~ (H y H1 H2) as [_ [_ [[H3 _] _]]]. *)
+(*   apply* (H3 x U). *)
+(*   pick_fresh y. assert (y \notin L) by auto. *)
+(*   assert (y \notin DFv e) by auto. *)
+(*   destruct~ (H y H1 H2) as [_ [_ [[_ H3] _]]]. *)
+(*   apply* (H3 x T U). *)
   
-  pick_fresh x. assert (x \notin L) by auto.
-  assert (x \notin DFv e) by auto.
-  destruct~ (H x H0 H1) as [_ [_ [_ [H2 _]]]].
-Qed.
+(*   pick_fresh x. assert (x \notin L) by auto. *)
+(*   assert (x \notin DFv e) by auto. *)
+(*   destruct~ (H x H0 H1) as [_ [_ [_ [H2 _]]]]. *)
+(* Qed. *)
 
-Lemma regular_dgen : forall E t s, DGen E t s ->
-  (DWf E /\ ok E /\ contains_terms E /\ DTerm t /\ DTermTy s).
-Proof.
-  apply dgen_induct with
-  (P := fun m E t T (_ : DTyping m E t T) => DWf E /\ ok E /\ contains_terms E /\ DTerm t /\ DTerm T)
-  (P0 := fun E t (_ : DWfTyp E t) => DWf E /\ ok E /\ contains_terms E /\ DTermTy t)
-  (P1 := fun E (_ : DWf E) => ok E /\ contains_terms E)
-  (P2 := fun E t T (_ : DInst E t T) => DWf E /\ ok E /\ contains_terms E /\ DTerm T);
-    unfolds contains_terms; intros; splits*.
-  
-  pick_fresh x. assert (x \notin L) by auto.
-  destruct (H x H0) as [H1 [_ [_ _]]].
-  inversion* H1. false* empty_push_inv.
-  destruct (eq_push_inv H2) as [_ [_ Eq]]. subst*.
-  destruct (eq_push_inv H2) as [_ [_ Eq]]. subst*.
-  destruct (eq_push_inv H2) as [_ [_ Eq]]. subst*.
+(* Hint Extern 1 (DTerm ?t) => match goal with *)
+(*   | H: DTyping _ _ t _ |- _ => apply (proj32 (proj33 (regular_dtyping H))) *)
+(*   | H: DTyping _ _ _ t |- _ => apply (proj33 (proj33 (regular_dtyping H))) *)
+(*   end. *)
 
-  pick_fresh x. assert (x \notin L) by auto.
-  destruct~ (H x H0) as [_ [H1 [_ _]]].
+(* Hint Extern 1 (DTermTy ?s) => match goal with *)
+(*   | H: DGen _ _ s  |- _ => apply (proj33 (proj33 (regular_dgen H))) *)
+(*   | H: DWfTyp _ s  |- _ => apply (proj44 (regular_dwftyp H)) *)
+(*   end. *)
 
-  split; intros.
-  pick_fresh y. assert (y \notin L) by auto.
-  destruct~ (H y H1) as [_ [_ [[H2 _] _]]].
-  apply* (H2 x U).
-  pick_fresh y. assert (y \notin L) by auto.
-  destruct~ (H y H1) as [_ [_ [[_ H2] _]]].
-  apply* (H2 x T U).
-  
-  intros. false* binds_empty_inv.
-  intros. false* binds_empty_inv.
+(* Lemma dok_from_wf : forall E, DWf E -> ok E. *)
+(* Proof. *)
+(*   induction 1. auto. autos* (regular_dtyping H1). *)
+(*   autos* (regular_dtyping H2). *)
+(*   autos* (regular_dwftyp H1). *)
+(* Qed. *)
 
-  intros. destruct (binds_push_inv H1) as [[? ?]|[? ?]].
-  injection H3; intros. subst*.
-  destruct H as [_ [H4 _]].
-  apply H4 with (x := x0). auto.
+(* Hint Extern 1 (ok ?E) => match goal with *)
+(*   | H: DWf E |- _ => apply (dok_from_wf H) *)
+(*   end. *)
 
-  intros. destruct (binds_push_inv H1) as [[? ?]|[? ?]].
-  false*. destruct H as [_ [_ H4]].
-  apply H4 with (x := x0). auto.
+(* Hint Extern 1 (DWf ?E) => match goal with *)
+(*   | H: DTyping _ E _ _ |- _ => apply (proj1 (regular_dtyping H)) *)
+(*   | H: DInst E _ _    |- _ => apply (proj1 (regular_dinst H)) *)
+(*   | H: DGen E _ _     |- _ => apply (proj1 (regular_dgen H)) *)
+(*   | H: DWfTyp E _     |- _ => apply (proj1 (regular_dwftyp H))    *)
+(*   end. *)
 
-  intros. destruct (binds_push_inv H2) as [[? ?]|[? ?]].
-  false*. destruct H as [_ [H5 _]].
-  apply H5 with (x := x0). auto.
+(* Lemma dwf_push_inv : forall E x U, *)
+(*   DWf (E & x ~ DC_Typ U) -> DWf E /\ DTermTy U. *)
+(* Proof. *)
+(*   introv W. inversions W.  *)
+(*   false (empty_push_inv H0). *)
+(*   destruct (eq_push_inv H) as [? [? ?]]. *)
+(*   false*. *)
+(*   destruct (eq_push_inv H) as [? [? ?]]. *)
+(*   injection H4; intros. *)
+(*   subst~. *)
+(*   destruct (eq_push_inv H) as [? [? ?]]. *)
+(*   false*. *)
+(*   destruct (eq_push_inv H) as [? [? ?]]. *)
+(*   false*. *)
+(* Qed. *)
 
-  intros. destruct (binds_push_inv H2) as [[? ?]|[? ?]].
-  injection H4; intros. subst*.
-  destruct H as [_ [_ H5]].
-  apply H5 with (x := x0). auto.
+(* Lemma dterm_from_binds_in_wf : forall x E U, *)
+(*   DWf E -> binds x (DC_Typ U) E -> DTerm U. *)
+(* Proof. *)
+(*   introv W Has. gen E. induction E using env_ind; intros. *)
+(*   false* binds_empty_inv. *)
+(*   destruct (binds_push_inv Has) as [[? ?]|[? ?]]. *)
+(*   subst~. destruct~ (dwf_push_inv W). *)
+(*   apply* IHE. *)
+(*   inversions* W. false* empty_push_inv. *)
+(*   destruct (eq_push_inv H1) as [_ [_ Eq]]. subst*. *)
+(*   destruct (eq_push_inv H1) as [_ [_ Eq]]. subst*. *)
+(*   destruct (eq_push_inv H1) as [_ [_ Eq]]. subst*. *)
+(* Qed. *)
 
-  intros. destruct (binds_push_inv H2) as [[? ?]|[? ?]].
-  false*. destruct H as [_ [H5 _]].
-  apply H5 with (x := x0). auto.
+(* Hint Extern 1 (DTerm ?t) => match goal with *)
+(*   H: binds ?x (DC_Typ t) ?E |- _ => apply (@dterm_from_binds_in_wf x E) *)
+(*   end. *)
 
-  intros. destruct (binds_push_inv H2) as [[? ?]|[? ?]].
-  injection H4; intros. subst*.
-  pick_fresh y. assert (y \notin L) by auto.
-  destruct (H1 y H3) as [_ [_ H5]].
-  destruct (H5 x (s ^' y) t). auto. split*.
-  destruct H as [_ [_ H5]].
-  apply H5 with (x := x0). auto.
+(* Lemma dwf_left : forall E F : DCtx, *)
+(*   DWf (E & F) -> DWf E. *)
+(* Proof. *)
+(*   intros. induction F using env_ind. *)
+(*   rewrite~ concat_empty_r in H. *)
+(*   rewrite concat_assoc in H. *)
+(*    inversions H. false (empty_push_inv H1). *)
+(*    destruct (eq_push_inv H0) as [? [? ?]]. subst~.  *)
+(*    destruct (eq_push_inv H0) as [? [? ?]]. subst~.  *)
+(*    destruct (eq_push_inv H0) as [? [? ?]]. subst~.  *)
+(* Qed. *)
 
-  pick_fresh x. assert (x \notin L) by auto.
-  assert (x \notin DFv e) by auto.
-  destruct (H x H0 H1) as [H2 [_ [_ _]]].
-  inversion* H2. false* empty_push_inv.
-  destruct (eq_push_inv H3) as [_ [_ Eq]]. subst*.
-  destruct (eq_push_inv H3) as [_ [_ Eq]]. subst*.
-  destruct (eq_push_inv H3) as [_ [_ Eq]]. subst*.
-
-  pick_fresh x. assert (x \notin L) by auto.
-  assert (x \notin DFv e) by auto.
-  destruct~ (H x H0 H1) as [_ [H2 [_ _]]].
-
-  split; intros.
-  pick_fresh y. assert (y \notin L) by auto.
-  assert (y \notin DFv e) by auto.
-  destruct~ (H y H1 H2) as [_ [_ [[H3 _] _]]].
-  apply* (H3 x U).
-  pick_fresh y. assert (y \notin L) by auto.
-  assert (y \notin DFv e) by auto.
-  destruct~ (H y H1 H2) as [_ [_ [[_ H3] _]]].
-  apply* (H3 x T U).
-  
-  pick_fresh x. assert (x \notin L) by auto.
-  assert (x \notin DFv e) by auto.
-  destruct~ (H x H0 H1) as [_ [_ [_ [H2 _]]]].
-Qed.
-
-Lemma regular_dwftyp : forall E t, DWfTyp E t ->
-  (DWf E /\ ok E /\ contains_terms E /\ DTermTy t).
-Proof.
-  apply dwftyp_induct with
-  (P := fun m E t T (_ : DTyping m E t T) => DWf E /\ ok E /\ contains_terms E /\ DTerm t /\ DTerm T)
-  (P1 := fun E (_ : DWf E) => ok E /\ contains_terms E)
-  (P2 := fun E t T (_ : DInst E t T) => DWf E /\ ok E /\ contains_terms E /\ DTerm T)
-  (P3 := fun E t T(_ : DGen E t T) => DWf E /\ ok E /\ contains_terms E /\ DTerm t /\ DTermTy T); 
-    unfolds contains_terms; intros; splits*.
-  
-  pick_fresh x. assert (x \notin L) by auto.
-  destruct (H x H0) as [H1 [_ [_ _]]].
-  inversion* H1. false* empty_push_inv.
-  destruct (eq_push_inv H2) as [_ [_ Eq]]. subst*.
-  destruct (eq_push_inv H2) as [_ [_ Eq]]. subst*.
-  destruct (eq_push_inv H2) as [_ [_ Eq]]. subst*.
-
-  pick_fresh x. assert (x \notin L) by auto.
-  destruct~ (H x H0) as [_ [H1 [_ _]]].
-
-  split; intros.
-  pick_fresh y. assert (y \notin L) by auto.
-  destruct~ (H y H1) as (_ & _ & (H2 & _) & _).
-  apply* (H2 x U).
-  pick_fresh y. assert (y \notin L) by auto.
-  destruct~ (H y H1) as (_ & _ & (_ & H2) & _).
-  apply* (H2 x T U). 
-  
-  intros. false* binds_empty_inv.
-  intros. false* binds_empty_inv.
-
-  intros. destruct (binds_push_inv H1) as [[? ?]|[? ?]].
-  injection H3; intros. subst*.
-  destruct H as [_ [H4 _]].
-  apply H4 with (x := x0). auto.
-
-  intros. destruct (binds_push_inv H1) as [[? ?]|[? ?]].
-  false*. destruct H as [_ [_ H4]].
-  apply H4 with (x := x0). auto.
-
-  intros. destruct (binds_push_inv H2) as [[? ?]|[? ?]].
-  false*. destruct H as [_ [H5 _]].
-  apply H5 with (x := x0). auto.
-
-  intros. destruct (binds_push_inv H2) as [[? ?]|[? ?]].
-  injection H4; intros. subst*.
-  destruct H as [_ [_ H5]].
-  apply H5 with (x := x0). auto.
-
-  intros. destruct (binds_push_inv H2) as [[? ?]|[? ?]].
-  false*. destruct H as [_ [H5 _]].
-  apply H5 with (x := x0). auto.
-
-  intros. destruct (binds_push_inv H2) as [[? ?]|[? ?]].
-  injection H4; intros. subst*.
-  pick_fresh y. assert (y \notin L) by auto.
-  destruct (H1 y H3) as [_ [_ H5]].
-  destruct (H5 x (s ^' y) t). auto. split*.
-  destruct H as [_ [_ H5]].
-  apply H5 with (x := x0). auto.
-
-  pick_fresh x. assert (x \notin L) by auto.
-  assert (x \notin DFv e) by auto.
-  destruct (H x H0 H1) as [H2 [_ [_ _]]].
-  inversion* H2. false* empty_push_inv.
-  destruct (eq_push_inv H3) as [_ [_ Eq]]. subst*.
-  destruct (eq_push_inv H3) as [_ [_ Eq]]. subst*.
-  destruct (eq_push_inv H3) as [_ [_ Eq]]. subst*.
-
-  pick_fresh x. assert (x \notin L) by auto.
-  assert (x \notin DFv e) by auto.
-  destruct~ (H x H0 H1) as [_ [H2 [_ _]]].
-
-  split; intros.
-  pick_fresh y. assert (y \notin L) by auto.
-  assert (y \notin DFv e) by auto.
-  destruct~ (H y H1 H2) as [_ [_ [[H3 _] _]]].
-  apply* (H3 x U).
-  pick_fresh y. assert (y \notin L) by auto.
-  assert (y \notin DFv e) by auto.
-  destruct~ (H y H1 H2) as [_ [_ [[_ H3] _]]].
-  apply* (H3 x T U).
-  
-  pick_fresh x. assert (x \notin L) by auto.
-  assert (x \notin DFv e) by auto.
-  destruct~ (H x H0 H1) as [_ [_ [_ [H2 _]]]].
-Qed.
-
-Hint Extern 1 (DTerm ?t) => match goal with
-  | H: DTyping _ _ t _ |- _ => apply (proj32 (proj33 (regular_dtyping H)))
-  | H: DTyping _ _ _ t |- _ => apply (proj33 (proj33 (regular_dtyping H)))
-  | H: DInst _ _ t    |- _ => apply (proj44 (regular_dinst H))
-  | H: DGen _ t _     |- _ => apply (proj32 (proj33 (regular_dgen H)))
-  end.
-
-Hint Extern 1 (DTermTy ?s) => match goal with
-  | H: DGen _ _ s  |- _ => apply (proj33 (proj33 (regular_dgen H)))
-  | H: DWfTyp _ s  |- _ => apply (proj44 (regular_dwftyp H))
-  end.
-
-Lemma dok_from_wf : forall E, DWf E -> ok E.
-Proof.
-  induction 1. auto. autos* (regular_dtyping H1).
-  autos* (regular_dtyping H2).
-  autos* (regular_dwftyp H1).
-Qed.
-
-Hint Extern 1 (ok ?E) => match goal with
-  | H: DWf E |- _ => apply (dok_from_wf H)
-  end.
-
-Hint Extern 1 (DWf ?E) => match goal with
-  | H: DTyping _ E _ _ |- _ => apply (proj1 (regular_dtyping H))
-  | H: DInst E _ _    |- _ => apply (proj1 (regular_dinst H))
-  | H: DGen E _ _     |- _ => apply (proj1 (regular_dgen H))
-  | H: DWfTyp E _     |- _ => apply (proj1 (regular_dwftyp H))   
-  end.
-
-Lemma dwf_push_inv : forall E x U,
-  DWf (E & x ~ DC_Typ U) -> DWf E /\ DTerm U.
-Proof.
-  introv W. inversions W. 
-  false (empty_push_inv H0).
-  destruct (eq_push_inv H) as [? [? ?]].
-  injection H4; intros.
-  subst~.
-  destruct (eq_push_inv H) as [? [? ?]].
-  false*.
-  destruct (eq_push_inv H) as [? [? ?]].
-  false*.
-Qed.
-
-Lemma dterm_from_binds_in_wf : forall x E U,
-  DWf E -> binds x (DC_Typ U) E -> DTerm U.
-Proof.
-  introv W Has. gen E. induction E using env_ind; intros.
-  false* binds_empty_inv.
-  destruct (binds_push_inv Has) as [[? ?]|[? ?]].
-  subst~. destruct~ (dwf_push_inv W).
-  apply* IHE.
-  inversions* W. false* empty_push_inv.
-  destruct (eq_push_inv H1) as [_ [_ Eq]]. subst*.
-  destruct (eq_push_inv H1) as [_ [_ Eq]]. subst*.
-  destruct (eq_push_inv H1) as [_ [_ Eq]]. subst*.
-Qed.
-
-Hint Extern 1 (DTerm ?t) => match goal with
-  H: binds ?x (DC_Typ t) ?E |- _ => apply (@dterm_from_binds_in_wf x E)
-  end.
-
-Lemma dwf_left : forall E F : DCtx,
-  DWf (E & F) -> DWf E.
-Proof.
-  intros. induction F using env_ind.
-  rewrite~ concat_empty_r in H.
-  rewrite concat_assoc in H.
-   inversions H. false (empty_push_inv H1).
-   destruct (eq_push_inv H0) as [? [? ?]]. subst~. 
-   destruct (eq_push_inv H0) as [? [? ?]]. subst~. 
-   destruct (eq_push_inv H0) as [? [? ?]]. subst~. 
-Qed.
-
-Implicit Arguments dwf_left [E F].
+(* Implicit Arguments dwf_left [E F]. *)
 
 (** Freshness *)
 
-Lemma dfv_open_var : forall y x t,
-  x <> y -> x \notin DFv (t ^ y) -> x \notin DFv t.
-Proof.
-  introv Neq. unfold DOpen. generalize 0. 
-  induction t; simpl; intros; try notin_solve.
-  specializes IHt1 n. auto. specializes IHt2 n. auto.
-  specializes IHt (S n). auto.
-  specializes IHt1 n. auto. specializes IHt2 (S n). auto.
-  specializes IHt1 n. auto. specializes IHt2 (S n). auto.
-  specializes IHt n. auto.
-  specializes IHt n. auto.
-  specializes IHt1 n. auto. specializes IHt2 n. auto.
-Qed.
+(* Lemma dfv_open_var : forall y x t, *)
+(*   x <> y -> x \notin DFv (t ^ y) -> x \notin DFv t. *)
+(* Proof. *)
+(*   introv Neq. unfold DOpen. generalize 0.  *)
+(*   induction t; simpl; intros; try notin_solve. *)
+(*   specializes IHt1 n. auto. specializes IHt2 n. auto. *)
+(*   specializes IHt (S n). auto. *)
+(*   specializes IHt1 n. auto. specializes IHt2 (S n). auto. *)
+(*   specializes IHt1 n. auto. specializes IHt2 (S n). auto. *)
+(*   specializes IHt n. auto. *)
+(*   specializes IHt n. auto. *)
+(*   specializes IHt1 n. auto. specializes IHt2 n. auto. *)
+(* Qed. *)
 
-Lemma dtyping_fresh : forall m x E t T,
-    DTyping m E t T -> x # E -> x \notin DFv t
-with dgen_fresh : forall x E t s,
-    DGen E t s -> x # E -> x \notin DFv t.
-Proof.
-  introv Typ.
-  induction Typ; simpls; intros.
-  auto.
-  rewrite notin_singleton. intro. subst. applys binds_fresh_inv H0 H1.
-  rewrite notin_singleton. intro. subst. applys binds_fresh_inv H0 H2.
-  lets: (IHTyp1 H). lets: (IHTyp2 H). auto.
-  pick_fresh y. apply* (@dfv_open_var y).
-  lets: (IHTyp1 H). lets: (IHTyp2 H). auto.
-  pick_fresh y. notin_simpl.
-  apply* dgen_fresh.
-  apply* (@dfv_open_var y).
-  pick_fresh y. notin_simpl. auto. apply* (@dfv_open_var y).
-  lets: (IHTyp H0). auto.
-  lets: (IHTyp H0). auto.
-  pick_fresh y. notin_simpl. auto. apply* (@dfv_open_var y).
-  pick_fresh y. notin_simpl.
-  apply* dgen_fresh.
-  apply* (@dfv_open_var y).
-  lets: (IHTyp H0). auto.
-  lets: (IHTyp H). auto.
+(* Lemma dtyping_fresh : forall m x E t T, *)
+(*     DTyping m E t T -> x # E -> x \notin DFv t *)
+(* with dgen_fresh : forall x E t s, *)
+(*     DGen E t s -> x # E -> x \notin DFv t. *)
+(* Proof. *)
+(*   introv Typ. *)
+(*   induction Typ; simpls; intros. *)
+(*   auto. *)
+(*   rewrite notin_singleton. intro. subst. applys binds_fresh_inv H0 H1. *)
+(*   rewrite notin_singleton. intro. subst. applys binds_fresh_inv H0 H2. *)
+(*   lets: (IHTyp1 H). lets: (IHTyp2 H). auto. *)
+(*   pick_fresh y. apply* (@dfv_open_var y). *)
+(*   lets: (IHTyp1 H). lets: (IHTyp2 H). auto. *)
+(*   pick_fresh y. notin_simpl. *)
+(*   apply* dgen_fresh. *)
+(*   apply* (@dfv_open_var y). *)
+(*   pick_fresh y. notin_simpl. auto. apply* (@dfv_open_var y). *)
+(*   lets: (IHTyp H0). auto. *)
+(*   lets: (IHTyp H0). auto. *)
+(*   pick_fresh y. notin_simpl. auto. apply* (@dfv_open_var y). *)
+(*   pick_fresh y. notin_simpl. *)
+(*   apply* dgen_fresh. *)
+(*   apply* (@dfv_open_var y). *)
+(*   lets: (IHTyp H0). auto. *)
+(*   lets: (IHTyp H). auto. *)
  
-  introv Gen.
-  induction Gen; simpls; intros.
-  apply* dtyping_fresh.
-  pick_fresh y. apply* H0.
-Qed.
+(*   introv Gen. *)
+(*   induction Gen; simpls; intros. *)
+(*   apply* dtyping_fresh. *)
+(*   pick_fresh y. apply* H0. *)
+(* Qed. *)
 
-Lemma notin_dfv_from_dwf : forall E F x V,
-  DWf (E & x ~ DC_Typ V & F) -> x \notin DFv V.
-Proof.
-  intros.
-  lets W: (dwf_left H). inversions W.
-  false (empty_push_inv H1).
-  destruct (eq_push_inv H0) as [? [? ?]].
-  injection H5. intros.
-  subst~.
-  apply* dtyping_fresh.
-  destruct (eq_push_inv H0) as [? [? ?]].
-  false*.
-  destruct (eq_push_inv H0) as [? [? ?]].
-  false*.
-Qed.
+(* Lemma notin_dfv_from_dwf : forall E F x V, *)
+(*   DWf (E & x ~ DC_Typ V & F) -> x \notin DFv V. *)
+(* Proof. *)
+(*   intros. *)
+(*   lets W: (dwf_left H). inversions W. *)
+(*   false (empty_push_inv H1). *)
+(*   destruct (eq_push_inv H0) as [? [? ?]]. *)
+(*   injection H5. intros. *)
+(*   subst~. *)
+(*   apply* dtyping_fresh. *)
+(*   destruct (eq_push_inv H0) as [? [? ?]]. *)
+(*   false*. *)
+(*   destruct (eq_push_inv H0) as [? [? ?]]. *)
+(*   false*. *)
+(* Qed. *)
 
-Lemma notin_dfv_from_binds : forall x y U E,
-  DWf E -> binds y (DC_Typ U) E -> x # E -> x \notin DFv U.
-Proof.
-  induction E using env_ind; intros.
-  false* binds_empty_inv.
-  destruct v.
-  destruct (dwf_push_inv H).
-  destruct (binds_push_inv H0) as [[? ?]|[? ?]]; subst.
-  inversions H. false* (empty_push_inv H6).
-  injection H5; intros; subst.
-  destruct (eq_push_inv H4) as [? [? ?]]. subst~. 
-  injection H9; intros; subst.
-  apply dtyping_fresh with (m := Chk)(E := E)(T := DE_Star).
-  auto. auto.   
-  destruct (eq_push_inv H4) as [? [? ?]]. false*.
-  destruct (eq_push_inv H4) as [? [? ?]]. false*.
-  apply* IHE.
-  destruct (binds_push_inv H0) as [[? ?]|[? ?]]; subst.
-  false*.
-  inversions H. false* (empty_push_inv H5).
-  destruct (eq_push_inv H4) as [? [? ?]]. false*. 
-  destruct (eq_push_inv H4) as [? [? ?]]; subst~.
-  destruct (eq_push_inv H4) as [? [? ?]]; subst~.
-Qed.
+(* Lemma notin_dfv_from_binds : forall x y U E, *)
+(*   DWf E -> binds y (DC_Typ U) E -> x # E -> x \notin DFv U. *)
+(* Proof. *)
+(*   induction E using env_ind; intros. *)
+(*   false* binds_empty_inv. *)
+(*   destruct v. *)
+(*   destruct (dwf_push_inv H). *)
+(*   destruct (binds_push_inv H0) as [[? ?]|[? ?]]; subst. *)
+(*   inversions H. false* (empty_push_inv H6). *)
+(*   injection H5; intros; subst. *)
+(*   destruct (eq_push_inv H4) as [? [? ?]]. subst~.  *)
+(*   injection H9; intros; subst. *)
+(*   apply dtyping_fresh with (m := Chk)(E := E)(T := DE_Star). *)
+(*   auto. auto.    *)
+(*   destruct (eq_push_inv H4) as [? [? ?]]. false*. *)
+(*   destruct (eq_push_inv H4) as [? [? ?]]. false*. *)
+(*   apply* IHE. *)
+(*   destruct (binds_push_inv H0) as [[? ?]|[? ?]]; subst. *)
+(*   false*. *)
+(*   inversions H. false* (empty_push_inv H5). *)
+(*   destruct (eq_push_inv H4) as [? [? ?]]. false*.  *)
+(*   destruct (eq_push_inv H4) as [? [? ?]]; subst~. *)
+(*   destruct (eq_push_inv H4) as [? [? ?]]; subst~. *)
+(* Qed. *)
 
-Lemma notin_dfv_from_binds' : forall E F x V y U,
-  DWf (E & x ~ DC_Typ V & F) -> binds y (DC_Typ U) E -> x \notin DFv U.
-Proof.
-  intros. lets W: (dwf_left H). inversions keep W.
-  false (empty_push_inv H2). 
-  destruct (eq_push_inv H1) as [? [? ?]]. subst~. 
-  lets W': (dwf_left W). apply* notin_dfv_from_binds.
-  destruct (eq_push_inv H1) as [? [? ?]]. false*.
-  destruct (eq_push_inv H1) as [? [? ?]]. false*.
-Qed.
+(* Lemma notin_dfv_from_binds' : forall E F x V y U, *)
+(*   DWf (E & x ~ DC_Typ V & F) -> binds y (DC_Typ U) E -> x \notin DFv U. *)
+(* Proof. *)
+(*   intros. lets W: (dwf_left H). inversions keep W. *)
+(*   false (empty_push_inv H2).  *)
+(*   destruct (eq_push_inv H1) as [? [? ?]]. subst~.  *)
+(*   lets W': (dwf_left W). apply* notin_dfv_from_binds. *)
+(*   destruct (eq_push_inv H1) as [? [? ?]]. false*. *)
+(*   destruct (eq_push_inv H1) as [? [? ?]]. false*. *)
+(* Qed. *)
 
-Hint Extern 1 (?x \notin DFv ?V) => 
-  match goal with H: DWf (?E & x ~ DC_Typ V & ?F) |- _ =>
-    apply (@notin_dfv_from_dwf E F) end.
+(* Hint Extern 1 (?x \notin DFv ?V) =>  *)
+(*   match goal with H: DWf (?E & x ~ DC_Typ V & ?F) |- _ => *)
+(*     apply (@notin_dfv_from_dwf E F) end. *)
 
-Hint Extern 1 (?x \notin DFv ?U) => 
-  match goal with H: DWf (?E & x ~ DC_Typ ?V & ?F), B: binds ?y U ?E |- _ =>
-    apply (@notin_dfv_from_binds' E F x V y) end.
-
+(* Hint Extern 1 (?x \notin DFv ?U) =>  *)
+(*   match goal with H: DWf (?E & x ~ DC_Typ ?V & ?F), B: binds ?y U ?E |- _ => *)
+(*     apply (@notin_dfv_from_binds' E F x V y) end. *)
